ver2/checker.v
@@ -19,8 +19,14 @@ Import SymbolicExecution.
 Require Import FORVES.storage_ops_solvers.
 Import StorageOpsSolvers.
 
+Require Import FORVES.storage_ops_solvers_impl.
+Import StorageOpsSolversImpl.
+
 Require Import FORVES.memory_ops_solvers.
 Import MemoryOpsSolvers.
+
+Require Import FORVES.memory_ops_solvers_impl.
+Import MemoryOpsSolversImpl.
 
 Require Import FORVES.symbolic_state_cmp.
 Import SymbolicStateCmp.
