ver2/memory_ops_solvers_impl.v
@@ -1,0 +1,104 @@
+Require Import Arith.  
+Require Import Nat.
+Require Import Bool.
+Require Import bbv.Word.
+Require Import Coq.NArith.NArith.
+Require Import List.
+Import ListNotations.
+Require Import Coq.Logic.FunctionalExtensionality.
+
+Require Import FORVES.constants.
+Import Constants.
+
+Require Import FORVES.program.
+Import Program.
+
+Require Import FORVES.execution_state.
+Import ExecutionState.
+
+Require Import FORVES.stack_operation_instructions.
+Import StackOpInstrs.
+
+Require Import FORVES.misc.
+Import Misc.
+
+Require Import FORVES.symbolic_state.
+Import SymbolicState.
+
+Require Import FORVES.symbolic_state_eval.
+Import SymbolicStateEval.
+
+Require Import FORVES.valid_symbolic_state.
+Import ValidSymbolicState.
+
+Require Import FORVES.memory_ops_solvers.
+Import MemoryOpsSolvers.
+
+Require Import FORVES.symbolic_state_cmp.
+Import SymbolicStateCmp.
+
+Module MemoryOpsSolversImpl.
+
+(* Doesn't check the memory for the value, just returns an abstract load *)
+Definition basic_mload_solver: mload_solver_type :=
+  fun (soffset: sstack_val) =>
+  fun (smem: smemory) =>
+  fun (instk_height: nat) =>
+  fun (m: smap) =>
+  fun (ops: stack_op_instr_map) =>
+  SymMLOAD soffset smem.
+
+Lemma basic_mload_solver_snd: mload_solver_snd basic_mload_solver.
+Admitted.
+
+(* Doesn't check the memory, just appends the abstract store *)
+Definition basic_smemory_updater: smemory_updater_type :=
+  fun (update: memory_update sstack_val) =>
+  fun (smem: smemory) =>
+  fun (instk_height: nat) =>
+  fun (m: smap) =>
+  fun (ops: stack_op_instr_map) =>
+  (update::smem).
+
+Lemma basic_smemory_updater_snd: smemory_updater_snd basic_smemory_updater.
+Admitted.
+
+
+Definition mstore_updates_do_not_overlap (soffset soffset': sstack_val) : bool :=
+  match soffset, soffset' with
+  | Val v1, Val v2 =>
+      let addr := (wordToN v1) in
+      let addr' := (wordToN v2) in
+      orb (addr+31 <? addr')%N (addr'+31 <? addr)%N
+  | _, _ => false
+  end.
+
+Definition mstore8_updates_do_not_overlap (soffset soffset': sstack_val) : bool :=
+  match soffset, soffset' with
+  | Val v1, Val v2 =>
+      let addr := (wordToN v1) in
+      let addr' := (wordToN v2) in
+      orb (addr <? addr')%N (addr'+31 <? addr)%N
+  | _, _ => false
+  end.
+
+Fixpoint adv_mload_solver (sstack_val_cmp: sstack_val_cmp_ext_1_t) (soffset: sstack_val) (smem: smemory) (instk_height: nat) (m: smap) (ops: stack_op_instr_map) :=
+  match smem with
+  | [] => SymMLOAD soffset []
+  | (U_MSTORE _ soffset' svalue)::smem' =>
+      if sstack_val_cmp (S (get_maxidx_smap m)) soffset soffset' (get_maxidx_smap m) (get_bindings_smap m) (get_maxidx_smap m) (get_bindings_smap m) instk_height ops then
+        SymBasicVal svalue
+      else
+        if mstore_updates_do_not_overlap soffset soffset' then
+          adv_mload_solver sstack_val_cmp soffset smem' instk_height m ops
+        else
+          SymMLOAD soffset' smem
+  | (U_MSTORE8 _ soffset' svalue)::smem' =>
+      if mstore8_updates_do_not_overlap soffset soffset' then
+        adv_mload_solver sstack_val_cmp soffset smem' instk_height m ops
+      else
+        SymMLOAD soffset' smem             
+  end.
+
+
+End MemoryOpsSolversImpl.
