ver2/storage_ops_solvers_soundness.v
@@ -1,0 +1,51 @@
+Require Import Arith.  
+Require Import Nat.
+Require Import Bool.
+Require Import bbv.Word.
+Require Import Coq.NArith.NArith.
+Require Import List.
+Import ListNotations.
+Require Import Coq.Logic.FunctionalExtensionality.
+
+Require Import FORVES.constants.
+Import Constants.
+
+Require Import FORVES.program.
+Import Program.
+
+Require Import FORVES.execution_state.
+Import ExecutionState.
+
+Require Import FORVES.stack_operation_instructions.
+Import StackOpInstrs.
+
+Require Import FORVES.misc.
+Import Misc.
+
+Require Import FORVES.symbolic_state.
+Import SymbolicState.
+
+Require Import FORVES.symbolic_state_eval.
+Import SymbolicStateEval.
+
+Require Import FORVES.valid_symbolic_state.
+Import ValidSymbolicState.
+
+Require Import FORVES.storage_ops_solvers.
+Import StorageOpsSolvers.
+
+Require Import FORVES.storage_ops_solvers_impl.
+Import StorageOpsSolversImpl.
+
+Module StorageOpsSolversSoundness.
+
+ 
+
+Lemma basic_sload_solver_snd: sload_solver_snd basic_sload_solver.
+Admitted.
+
+
+Lemma basic_sstorage_updater_snd: sstorage_updater_snd basic_sstorage_updater.
+Admitted.
+
+End StorageOpsSolversSoundness.
